WIP low => mid proof for PointAddIntoDest

src/specs/PointAddIntoDest.ec
@@ -31,9 +31,40 @@ module PointAddIntoDest = {
       RevertWithMessage.low((W256.of_int 30), (W256.of_int STRING (*pointAddIntoDest: ecAdd failed*)));
     }
   }
+
+  proc low'(p1, p2, dest) =
+  {
+    var _1, _5, _6, _9, _13, _14;
+    _1 <@ Primops.mload(p1);
+    _5 <@ Primops.mload(p1 + W256.of_int 32);
+    _6 <@ Primops.mload(p2);
+    _9 <@ Primops.mload(p2 + W256.of_int 32);
+    Primops.mstore(W256.of_int 0, _1);
+    Primops.mstore(W256.of_int 32, _5);
+    Primops.mstore(W256.of_int 64, _6);
+    Primops.mstore(W256.of_int 96, _9);
+    _13 <@ Primops.gas();
+    _14 <@ Primops.staticcall(_13, W256.of_int 6, W256.zero, W256.of_int 128, dest, W256.of_int 64);
+    if ((bool_of_uint256 (PurePrimops.iszero _14)))
+    {
+      RevertWithMessage.low((W256.of_int 30), (W256.of_int STRING (*pointAddIntoDest: ecAdd failed*)));
+    }
+  }
+
+  proc mid(x1 : int, y1 : int, x2 : int, y2 : int) : int * int = {
+    var x, y, x1_F, x2_F, y1_F, y2_F, result;
+      x1_F <- ZModField.inzmod x1;
+      y1_F <- ZModField.inzmod y1;
+      x2_F <- ZModField.inzmod x2;
+      y2_F <- ZModField.inzmod y2;
+      result <- ecAdd_precompile x1_F y1_F x2_F y2_F;
+      (x, y) <- odflt (ZModField.zero, ZModField.zero) result;
+      return (ZModField.asint x, ZModField.asint y);
+  }
 }.
 
 lemma pointAddIntoDest_extracted_equiv_low : equiv [
+
     Verifier_1261.usr_pointAddIntoDest ~ PointAddIntoDest.low :
       ={arg, glob PointAddIntoDest} ==>
       ={res, glob PointAddIntoDest}
@@ -44,3 +75,103 @@ proof.
   inline*. wp. skip. by progress.
   inline*. wp. skip. by progress.
 qed.
+
+lemma usr_pointAddIntoDest_low_matches_low' (p1 p2 dest : uint256) : equiv [
+    PointAddIntoDest.low ~ PointAddIntoDest.low':
+      ={arg, glob PointAddIntoDest} /\
+      arg{1} = (p1, p2, dest) /\
+        W256.of_int 128 < p1 /\ W256.of_int 128 < (p1 + W256.of_int 32) /\
+        W256.of_int 128 < p2 /\ W256.of_int 128 < (p2 + W256.of_int 32) ==>
+      ={res, glob PointAddIntoDest}
+    ].
+proof.
+  proc.
+  sim.
+  inline*. wp. skip. progress.
+
+  rewrite MemoryMap.load_store_diff.
+  have H' : p2{2} + W256.of_int 32 - W256.of_int 64 = p2{2} - W256.of_int 32. smt (@W256).
+  rewrite H'. admit.
+  admit.
+
+  rewrite MemoryMap.load_store_diff.
+  admit.
+  admit.
+
+  rewrite MemoryMap.load_store_diff.
+  admit.
+  admit.
+
+  reflexivity.
+
+  rewrite MemoryMap.load_store_diff.
+  admit.
+  admit.
+
+  rewrite MemoryMap.load_store_diff.
+  admit.
+  admit.
+
+  rewrite MemoryMap.load_store_diff.
+  admit.
+  admit.
+
+  reflexivity.
+qed.
+
+lemma PointAddIntoDest_mid_of_low (x1 x2 y1 y2 : int) (p1 p2 dest : uint256) : equiv [
+    PointAddIntoDest.low' ~ PointAddIntoDest.mid :
+    x1 < p /\ x2 < p /\ y1 < p /\ y2 < p /\
+    PurePrimops.mload Primops.memory{1} p1 = W256.of_int x1 /\
+    PurePrimops.mload Primops.memory{1} (p1 + W256.of_int 32) = W256.of_int y1 /\
+    PurePrimops.mload Primops.memory{1} p2 = W256.of_int x2 /\
+    PurePrimops.mload Primops.memory{1} (p2 + W256.of_int 32) = W256.of_int y2 /\
+      arg{1} = (p1, p2, dest) /\ arg{2} = (x1, y1, x2, y2)
+      ==>
+      (
+        exists (x y : F),
+        ecAdd_precompile (ZModField.inzmod x1) (ZModField.inzmod y1) (ZModField.inzmod x2) (ZModField.inzmod y2) = Some (x, y) /\
+        res{2} = (ZModField.asint x, ZModField.asint y) /\
+        PurePrimops.mload Primops.memory{1} dest = W256.of_int (ZModField.asint x) /\
+        PurePrimops.mload Primops.memory{1} (dest + W256.of_int 32) = W256.of_int (ZModField.asint y)
+      ) \/
+      (
+        ecAdd_precompile (ZModField.inzmod x1) (ZModField.inzmod y1) (ZModField.inzmod x2) (ZModField.inzmod y2) = None /\
+        res{2} = (0, 0) /\
+        PurePrimops.mload Primops.memory{1} dest = W256.zero /\
+        PurePrimops.mload Primops.memory{1} (dest + W256.of_int 32) = W256.zero
+      )
+    ]. proof.
+        exists* Primops.memory{1}.
+        elim* => memory.
+        proc.
+        seq 4 0 :
+    (
+      #pre /\
+      _1{1} = W256.of_int x1 /\
+      _5{1} = W256.of_int y1 /\
+      _6{1} = W256.of_int x2 /\
+      _5{1} = W256.of_int y1 /\
+      _9{1} = W256.of_int y2
+    ).
+    inline *. wp. skip. progress.
+    seq 5 0 : 
+    (
+      x1 < p /\
+      x2 < p /\
+      y1 < p /\
+      y2 < p /\
+      (p1{1}, p2{1}, dest{1}) = (p1, p2, dest) /\
+      (x1{2}, y1{2}, x2{2}, y2{2}) = (x1, y1, x2, y2) /\
+    _1{1} = (of_int x1)%W256 /\
+    _5{1} = (of_int y1)%W256 /\
+    _6{1} = (of_int x2)%W256 /\
+    _5{1} = (of_int y1)%W256 /\ _9{1} = (of_int y2)%W256 /\
+    Primops.memory{1} = PurePrimops.mstore (PurePrimops.mstore (PurePrimops.mstore (PurePrimops.mstore memory W256.zero _1{1}) (W256.of_int 32) _5{1}) (W256.of_int 64) _6{1}) (W256.of_int 96) _9{1}
+    ).
+        inline *. wp. skip. progress.
+        inline Primops.staticcall. sp.
+        rcondf{1} 1. progress. skip. progress. smt (@W256).
+        rcondt{1} 1. move=> &m. skip. progress.
+        inline Primops.mload. sp.
+        (* inline*. wp. skip. progress. *)
